new agreement spec

paxos/proof.dfy
@@ -104,107 +104,151 @@ lemma NextPreservesVakidityInv(c:Constants, v:Value, ds:DistrSys, ds':DistrSys)
 *****************************************************************************************/
 
 /* All correct processes decide the same value */
-predicate Agreement(c:Constants, ds:DistrSys, v:Value, b:Ballot) 
+predicate Agreement(c:Constants, ds:DistrSys) 
     requires c.WF()
     requires ds.WF(c)
 {
-    SomeProcessDecidedV(c, ds, v, b) ==> AllDecidedProcessesDecidesV(c, ds, v)
+    forall v, b, idx | c.ValidLdrIdx(idx) && LeaderIdxDecidedV(c, ds, idx, v, b) 
+    :: AllDecidedProcessesDecidesV(c, ds, v)
 }
 
-predicate SomeProcessDecidedV(c:Constants, ds:DistrSys, v:Value, b:Ballot) 
-    requires c.WF()
-    requires ds.WF(c)
+predicate LeaderIdxDecidedV(c:Constants, ds:DistrSys, idx:int, v:Value, b:Ballot) 
+    requires c.WF() && ds.WF(c)
+    requires c.ValidLdrIdx(idx)
 {
     && b != Bottom
-    && exists i :: 
-        && c.ValidLdrIdx(i) 
-        && ds.leaders[i].state == Decided 
-        && ds.leaders[i].val == v
-        && ds.leaders[i].ballot == b
+    && ds.leaders[idx].state == Decided 
+    && ds.leaders[idx].val == v
+    && ds.leaders[idx].ballot == b
 }
 
 
 /* Invariants for establishing Agreement */
-predicate Agreement_Inv(c:Constants, ds:DistrSys, v:Value, b:Ballot) 
+predicate Agreement_Inv(c:Constants, ds:DistrSys, b:Ballot) 
 {
     && c.WF()
     && ds.WF(c)
-    && Agreement(c, ds, v, b)
-    && Agreement_Inv_AcceptedByQuorum(c, ds, v, b)
-    && Agreement_Inv_Messages(c, ds, v, b)
-    && Agreement_Inv_P2Leaders(c, ds, v, b)
-}
-
-
-predicate Agreement_Inv_AcceptedByQuorum(c:Constants, ds:DistrSys, v:Value, b:Ballot) 
-    requires c.WF() && ds.WF(c)
-{
-    SomeProcessDecidedV(c, ds, v, b) ==> (
-        exists quorum ::
-            && QuorumOfAcceptors(c, quorum)
-            && AcceptedByQuroum(c, ds, quorum, v, b)
-    )
-}
-
-predicate AcceptedByQuroum(c:Constants, ds:DistrSys, q:set<int>, v:Value, b:Ballot) 
-    requires c.WF() && ds.WF(c)
-    requires QuorumOfAcceptors(c, q)
-{
-    forall idx | idx in q ::
-        && ds.acceptors[idx].accepted == v
-        && BalLtEq(b, ds.acceptors[idx].promised)
-}
-
-
-predicate Agreement_Inv_Messages(c:Constants, ds:DistrSys, v:Value, b:Ballot) 
-    requires c.WF() && ds.WF(c)
-{
-    SomeProcessDecidedV(c, ds, v, b) 
-    ==> 
-    (forall pkt | pkt in ds.network.sentPackets && BalLtEq(b, pkt.msg.bal)
-    :: ProposeAndPreemptContainsV(pkt.msg, v))
-}
-
-predicate ProposeAndPreemptContainsV(m:Message , v:Value) {
-    match m {
-        case Propose(bal, val) => val == v
-        case Preempt(bal, val) => val == v
-        case _ => true
-    }
-}
-
-predicate Agreement_Inv_P2Leaders(c:Constants, ds:DistrSys, v:Value, b:Ballot) 
-    requires c.WF() && ds.WF(c)
-{
-    SomeProcessDecidedV(c, ds, v, b) 
-    ==> 
-    (forall i | 
-        && c.ValidLdrIdx(i) 
-        && LeaderInPhase2(c, i, ds) 
-        && BalLtEq(b, ds.leaders[i].ballot)
-    :: ds.leaders[i].val == v)
+    && Agreement(c, ds)
 }
 
 
 /* Init ==> Agreement_Inv */
-lemma InitImpliesAgreementInv(c:Constants, ds:DistrSys, v:Value, b:Ballot) 
+lemma InitImpliesAgreementInv(c:Constants, ds:DistrSys, b:Ballot) 
     requires Init(c, ds)
-    ensures Agreement_Inv(c, ds, v, b)
+    ensures Agreement_Inv(c, ds, b)
 {}
 
 
 /* Agreement_Inv && Next ==> Agreement_Inv' */
-lemma NextPreservesAgreementInv(c:Constants, v:Value, b:Ballot, ds:DistrSys, ds':DistrSys) 
-    requires Agreement_Inv(c, ds, v, b)
+lemma NextPreservesAgreementInv(c:Constants, b:Ballot, ds:DistrSys, ds':DistrSys) 
+    requires Agreement_Inv(c, ds, b)
     requires Next(c, ds, ds')
-    ensures Agreement_Inv(c, ds', v, b)
+    ensures Agreement_Inv(c, ds', b)
 {
-    // TODO
-    assume false;
-    assert Agreement_Inv_AcceptedByQuorum(c, ds', v, b);
-    assert Agreement_Inv_Messages(c, ds', v, b);
-    assert Agreement_Inv_P2Leaders(c, ds', v, b);
-    assert Agreement(c, ds', v, b);
+    if exists v, b, i :: c.ValidLdrIdx(i) && LeaderIdxDecidedV(c, ds, i, v, b) {
+        // If someone has decided in ds
+        // TODO
+        assume false;
+        assert Agreement(c, ds');
+    } else {
+        // If no one has decided in ds
+        var src, recvIos, sendIos :| PaxosNextOneAgent(c, ds, ds', src, recvIos, sendIos);
+        if src.agt == Acc {
+            assert forall l | l in ds'.leaders :: !l.state.Decided?;
+            assert forall l | l in ds'.leaders :: !l.state.Decided?;
+            assert forall v, b, i | c.ValidLdrIdx(i) :: !LeaderIdxDecidedV(c, ds', i, v, b);
+            assert Agreement(c, ds');
+        } else {
+            // TODO
+            assume false;
+            assert Agreement(c, ds');
+        }
     }
+}
+
+
+
+
+
+
+/* Assumption that if v is decided with ballot b, then all values decided with ballots
+* b' >= b must be of v */
+predicate FutureProposalsInv(c:Constants, ds:DistrSys, i:int, v:Value, b:Ballot)
+    requires c.WF() && ds.WF(c)
+    requires c.ValidLdrIdx(i) 
+{
+    LeaderIdxDecidedV(c, ds, i, v, b) 
+    ==> 
+    (forall v', b', i' | 
+        && c.ValidLdrIdx(i') 
+        && BalLtEq(b, b') 
+        && LeaderIdxDecidedV(c, ds, i', v', b') 
+        :: v' == v)
+}
+
+
+lemma lemma_FutureProposalsInv(c:Constants, v:Value, i:int, b:Ballot, ds:DistrSys, ds':DistrSys)
+    requires c.WF() && ds.WF(c)
+    requires c.ValidLdrIdx(i) 
+    requires FutureProposalsInv(c, ds, i, v, b)
+    requires Next(c, ds, ds')
+    ensures FutureProposalsInv(c, ds', i, v, b);
+{
+    assume false;
+}
+
+
+
+
+
+
+// predicate Agreement_Inv_AcceptedByQuorum(c:Constants, ds:DistrSys, v:Value, b:Ballot) 
+//     requires c.WF() && ds.WF(c)
+// {
+//     SomeProcessDecidedV(c, ds, v, b) ==> (
+//         exists quorum ::
+//             && QuorumOfAcceptors(c, quorum)
+//             && AcceptedByQuroum(c, ds, quorum, v, b)
+//     )
+// }
+
+// predicate AcceptedByQuroum(c:Constants, ds:DistrSys, q:set<int>, v:Value, b:Ballot) 
+//     requires c.WF() && ds.WF(c)
+//     requires QuorumOfAcceptors(c, q)
+// {
+//     forall idx | idx in q ::
+//         && ds.acceptors[idx].accepted == v
+//         && BalLtEq(b, ds.acceptors[idx].promised)
+// }
+
+
+// predicate Agreement_Inv_Messages(c:Constants, ds:DistrSys, v:Value, b:Ballot) 
+//     requires c.WF() && ds.WF(c)
+// {
+//     SomeProcessDecidedV(c, ds, v, b) 
+//     ==> 
+//     (forall pkt | pkt in ds.network.sentPackets && BalLtEq(b, pkt.msg.bal)
+//     :: ProposeAndPreemptContainsV(pkt.msg, v))
+// }
+
+// predicate ProposeAndPreemptContainsV(m:Message , v:Value) {
+//     match m {
+//         case Propose(bal, val) => val == v
+//         case Preempt(bal, val) => val == v
+//         case _ => true
+//     }
+// }
+
+// predicate Agreement_Inv_P2Leaders(c:Constants, ds:DistrSys, v:Value, b:Ballot) 
+//     requires c.WF() && ds.WF(c)
+// {
+//     SomeProcessDecidedV(c, ds, v, b) 
+//     ==> 
+//     (forall i | 
+//         && c.ValidLdrIdx(i) 
+//         && LeaderInPhase2(c, i, ds) 
+//         && BalLtEq(b, ds.leaders[i].ballot)
+//     :: ds.leaders[i].val == v)
+// }
 
 }
